Finish Abs proof

Optimizations/Canonicalizations/AbsPhase.thy
@@ -130,6 +130,7 @@ lemma bit_invariant_not_mask':
   using assms
   by (metis (no_types, lifting) Groups.add_ac(2) bit_imp_le_length bit_take_bit_iff less_le mask_eq_exp_minus_1 take_bit_incr_eq_word)
 
+
 lemma negative_negation_is_positive:
   assumes "0 < b \<and> b \<le> 64"
   assumes "v \<noteq> take_bit b (min_int b)"
@@ -296,10 +297,102 @@ optimization AbsIdempotence:
   using intval_abs_simp abs_value_idempotence
   by (smt (verit, best) eval_bits_1_64 eval_unused_bits_zero intval_abs.elims new_int.simps unary_eval.simps(1) unfold_evaltree(2))
 
+thm_oracles AbsIdempotence
+
+lemma mod_plus_one:
+  fixes v :: "'a::len word"
+  assumes "0 < b \<and> b < LENGTH('a)"
+  assumes "v mod (2^b) < (2^b) - 1"
+  shows "v mod (2^b) + 1 = (v+1) mod (2^b)"
+proof -
+  have t1:"take_bit LENGTH('a) 2^b = 2^b"
+    by (smt (verit, ccfv_SIG) One_nat_def Suc_pred assms(1) bits_one_mod_two_eq_one bot_nat_0.extremum_strict less_Suc_numeral less_irrefl minus_mod_eq_div_mult minus_mod_eq_mult_div mult_div_mod_eq not_gr0 numeral_Bit0_div_2 numeral_code(1) of_nat_numeral of_nat_take_bit rel_simps(51) take_bit_Suc_0 take_bit_of_1 take_bit_rec)
+  have t2:"take_bit LENGTH('a) 2^LENGTH('a)-1 = 2^LENGTH('a)-1"
+    by (smt (verit, ccfv_SIG) One_nat_def Suc_pred assms(1) bits_one_mod_two_eq_one bot_nat_0.extremum_strict less_Suc_numeral less_irrefl minus_mod_eq_div_mult minus_mod_eq_mult_div mult_div_mod_eq not_gr0 numeral_Bit0_div_2 numeral_code(1) of_nat_numeral of_nat_take_bit rel_simps(51) take_bit_Suc_0 take_bit_of_1 take_bit_rec)
+  (*have "2^b < 2^LENGTH('a)-1"
+    using t1 t2 assms(1) sledgehammer*)
+  then have "v mod (2^b) + 1 < (2^b)"
+    by (smt (verit) assms(1) assms(2) exp_eq_zero_iff not_less one_le_power uint_2p uint_arith_simps(2) uint_arith_simps(5) uint_word_ariths(2) uint_word_ariths(8) word_greater_zero_iff zmod_le_nonneg_dividend)
+    then show ?thesis
+  using assms
+  by (metis ValueThms.take_bit_dist_addL take_bit_eq_word take_bit_mod)
+qed
+
+lemma
+  fixes v y :: "'a::len word"
+  assumes "0 < y \<and> y < 2^LENGTH('a)-1"
+  assumes "0 \<le> r \<and> r < y"
+  shows "((((v div y) * y)) div y) = (v div y)"
+  using assms
+  using div_lt' word_div_mult by blast
+
+
+lemma bit_invariant_modulo:
+  fixes v :: "'a::len word"
+  assumes "b > 0 \<and> b < LENGTH('a)"
+  assumes "v mod (2^b) \<noteq> (2^b) - 1"
+  shows "odd (v div (2^b)) = odd ((v+1) div (2^b))"
+proof -
+  have "(v mod 2^b) < 2^b"
+    by (metis and_mask_less_size assms(1) take_bit_eq_mask take_bit_mod wsst_TYs(3))
+  then have "(v mod 2^b) < (2^b) - 1"
+    using assms(2)
+    by (smt (verit, best) len_gt_0 less_le mod_pos_pos_trivial of_bool_eq(2) one_mod_2_pow_eq uint_arith_simps(2) uint_lt2p uint_word_ariths(8) uint_word_of_int wi_le word_arith_wis(2) word_mod_def word_sub_less_iff)
+  then have "(v mod 2^b) + 1 = (v+1) mod 2^b"
+    by (simp add: assms(1) mod_plus_one)
+  then have e: "(v div 2^b)*2^b + (v mod 2^b) + 1
+        = (v div 2^b)*2^b + ((v+1) mod 2^b)"
+    using assms by (simp)
+  have "of_bool (bit v b) = ((v div 2^b) mod 2)"
+    by (simp add: bit_iff_odd mod2_eq_if)
+  have "(((v + 1) div 2^b) mod 2) = ((((v div 2^b) * 2^b + v mod 2^b)+1) div 2^b) mod 2"
+    by presburger
+  then have a: "... = (((((v+1) div 2^b) * 2^b + (v+1) mod 2^b)) div 2^b) mod 2"
+    using assms
+    by presburger
+  then have b: "... = ((((v div 2^b) * 2^b + (v+1) mod 2^b)) div 2^b) mod 2"
+    using assms
+    using e by presburger
+  then have "... = (v div 2^b) mod 2"
+    using assms
+    by (smt (verit, del_insts) add_diff_cancel_right' e exp_eq_zero_iff minus_mod_eq_div_mult mult_div_le mult_div_mod_eq nonzero_mult_div_cancel_right not_less of_bool_eq(2) take_bit_int_less_exp take_bit_of_1 uint_2p uint_div uint_lt2p uint_mult_lem word_div_def word_greater_zero_iff)
+  then show ?thesis
+    by (metis b mod_div_decomp odd_iff_mod_2_eq_one)
+qed
+
+lemma bit_invariant_not_mask'':
+  fixes v :: "'a::len word"
+  assumes "0 < b \<and> b < LENGTH('a)"
+  assumes "take_bit b v \<noteq> mask b"
+  shows "bit v b = bit ((v + 1)) b"
+  using assms bit_invariant_modulo
+  by (metis bit_iff_odd mask_eq_exp_minus_1 take_bit_eq_mod)
+
+lemma positive_negation_is_positive:
+  assumes "0 < b \<and> b \<le> 64"
+  assumes "take_bit b v = v"    
+  assumes "b \<turnstile> 0 <j v"
+  shows "b \<turnstile> -v <j 0"
+  using assms take_bit_incr_eq
+proof -
+  have "\<not>(bit v (b-1))"
+    using assms(1) assms(3) jgt_zero_sign_bit by presburger
+  have "-v = (not v) + 1"
+    by (simp add: minus_eq_not_plus_1)
+  have "(bit (not v) (b-1))"
+    using \<open>\<not> bit v (b - 1)\<close> assms(1) bit_not_iff_eq by fastforce
+  also have nm: "take_bit (b-1) (not v) \<noteq> mask (b-1)"
+    by (metis (mono_tags, opaque_lifting) \<open>\<not> bit v (b - 1)\<close> assms(3) bit.compl_zero int_signed_value.simps less_le signed_take_bit_eq_if_positive signed_take_bit_of_0 take_bit_minus_one_eq_mask take_bit_not_take_bit take_bit_of_0 word_not_not)
+  ultimately have "(bit ((not v) + 1) (b-1))"
+    by (metis assms(1) assms(3) bit_imp_le_length bit_invariant_not_mask'' diff_is_0_eq le_simps(1) mask_0 max_int_mask max_int_max max_int_signed_2pow_signed not_less zero_less_diff)
+  then show ?thesis
+    using \<open>- v = not v + 1\<close> assms(1) jlt_zero_sign_bit by presburger
+qed
+
 lemma abs_value_negation: \<comment>\<open>Proof walked through in Brae's thesis Chap. 9\<close>
   assumes "0 < b \<and> b \<le> 64"
   assumes "take_bit b v = v"
-  shows "abs b (-v) = abs b v"
+  shows "abs b (take_bit b (-v)) = abs b v"
 proof (cases "v = take_bit b (min_int b)")
   case True
   then show ?thesis
@@ -315,348 +408,26 @@ next
     then show ?thesis proof (cases "b \<turnstile> 0 <j v")
       case True
       have "b \<turnstile> -v <j 0"
-        using notmin sorry
-      then show ?thesis sorry
+        using notmin positive_negation_is_positive
+        using True assms(1) assms(2) by blast
+      then show ?thesis
+        by (smt (verit) JavaWords.take_bit_dist_neg ValueThms.signed_take_take_bit abs.simps assms(1) int_signed_value.simps more_arith_simps(10) negative_negation_is_positive)
     next
       case False
-      then show ?thesis sorry
+      then show ?thesis
+        by (smt (verit, best) abs.simps abs_value_idempotence assms(1) assms(2) notzero signed_value_eq take_bit_of_0)
+
     qed
   qed
 qed
 
-text \<open>
-Note:
+optimization AbsNegation:
+  "abs(-x) \<longmapsto> abs(x)"
+  apply auto
+  using intval_abs_simp abs_value_negation
+  by (smt (verit, ccfv_threshold) eval_bits_1_64 eval_unused_bits_zero intval_abs.simps(1) intval_negate.elims new_int.simps unary_eval.simps(1) unfold_unary)
 
-We can't use @{const word_sless} for reasoning about @{const intval_less_than}.
-@{const word_sless} will always treat the $64^{th}$ bit as the sign flag
-while @{const intval_less_than} uses the $b^{th}$ bit depending on the size of the word.
-\<close>
-
-value "val[new_int 32 0 < new_int 32 4294967286]" \<comment> \<open>0 < -10 = False\<close>
-value "(0::int64) <s 4294967286" \<comment> \<open>0 < 4294967286 = True\<close>
-
-
-lemma signed_eqiv:
-  assumes "b > 0 \<and> b \<le> 64"
-  shows "val_to_bool (val[new_int b v < new_int b v']) = (int_signed_value b v < int_signed_value b v')"
-  using assms
-  by (metis (no_types, lifting) ValueThms.signed_take_take_bit bool_to_val.elims bool_to_val_bin.elims int_signed_value.simps intval_less_than.simps(1) new_int.simps one_neq_zero val_to_bool.simps(1))
-
-lemma val_abs_pos:
-  assumes "val_to_bool(val[(new_int b 0) < (new_int b v)])"
-  shows "intval_abs (new_int b v) = (new_int b v)"
-  using assms by force
-
-lemma val_abs_neg:
-  assumes "val_to_bool(val[(new_int b v) < (new_int b 0)])"
-  shows "intval_abs (new_int b v) = intval_negate (new_int b v)"
-  using assms by force
-
-lemma val_bool_unwrap:
-  "val_to_bool (bool_to_val v) = v"
-  by (metis bool_to_val.elims one_neq_zero val_to_bool.simps(1))
-
-
-lemma take_bit_64:
-  assumes "0 < b \<and> b \<le> 64"
-  assumes "take_bit b v = v"
-  shows "take_bit 64 v = take_bit b v"
-  using assms
-  by (metis min_def nle_le take_bit_take_bit)
-
-
-text \<open>
-A special value exists for the maximum negative integer as its negation is itself.
-We can define the value as @{term "(set_bit (b - 1) 0)::int64"} for any bit-width, b.
-\<close>
-
-value "(set_bit 1 0)::2 word" \<comment> \<open>2\<close>
-value "-(set_bit 1 0)::2 word" \<comment> \<open>2\<close>
-value "(set_bit 31 0)::32 word" \<comment> \<open>2147483648\<close>
-value "-(set_bit 31 0)::32 word" \<comment> \<open>2147483648\<close>
-
-
-lemma negative_def:
-  fixes v :: "'a::len word"
-  assumes "v <s 0"
-  shows "bit v (LENGTH('a) - 1)"
-  using assms
-  by (simp add: bit_last_iff word_sless_alt)
-
-lemma positive_def:
-  fixes v :: "'a::len word"
-  assumes "0 <s v"
-  shows "\<not>(bit v (LENGTH('a) - 1))"
-  using assms
-  by (simp add: bit_last_iff word_sless_alt)
-
-(*
-lemma invert1:
-  fixes v :: "'a::len word"
-  assumes "v <s 0"
-  assumes "v > (2^(LENGTH('a) - 1))"
-  shows "0 <s (-v)"
-proof -
-  have "-v = Word.Word (-(Word.rep v))"
-    by (metis uminus_word.abs_eq unsigned.abs_eq unsigned.rep_eq word_minus_def)
-  have "v < 0 \<longrightarrow> 0 < (-(Word.rep v))"
-    by auto
-  have negbit: "bit v (LENGTH('a) - 1)"
-    using assms(1) negative_def by blast
-  then have "0 <s (-v) = (0 < signed_take_bit (LENGTH('a) - 1) (Word.rep (-v)))"
-    unfolding word_sless_def apply simp
-    by (metis id_apply of_int_eq_id signed.rep_eq sint_0)
-  have "signed_take_bit (LENGTH('a) - 1) (Word.rep v) = (or (take_bit (LENGTH('a) - 1) (Word.rep v)) (not (mask (LENGTH('a) - 1))))"
-    using signed_take_bit_eq_if_negative negbit
-    by (metis bit_word.rep_eq)
-  then have "0 <s (-v) = (0 < (or (take_bit (LENGTH('a) - 1) (Word.rep (-v))) (not (mask (LENGTH('a) - 1)))))"
-    unfolding word_sless_def apply simp using signed_take_bit_eq_if_negative negbit sorry
-  have "0 < (-(Word.rep v) mod 2^(LENGTH('a) - 1)) \<longrightarrow> 0 <s (-v)"
-    unfolding word_sless_def sorry
-  then show ?thesis sorry
-qed
-
-value "1::1 word"
-value "2^(1 - 1)::1 word"
-value "bit (1::1 word) 1"
-
-lemma
-  fixes v :: "'a::len word"
-  shows "v \<ge> (2^(LENGTH('a) - 1)) \<Longrightarrow> bit v (LENGTH('a) - 1)"
-  sorry
-
-lemma negative_lower_bound:
-  fixes v :: "'a::len word"
-  assumes "v <s 0"
-  shows "v \<ge> (2^(LENGTH('a) - 1))"
-  using assms unfolding word_sless_def
-  apply auto sorry
-
-lemma invert:
-  fixes v :: "'a::len word"
-  assumes "v <s 0"
-  assumes "v \<noteq> (2^(LENGTH('a) - 1))"
-  shows "0 <s (-v)"
-  using invert1 assms negative_lower_bound order_less_le by blast
-*)
-
-lemma negative_lower_bound:
-  fixes v :: "'a::len word"
-  assumes "(2^(LENGTH('a) - 1)) <s v"
-  assumes "v <s 0"
-  shows "0 <s (-v)"
-  using assms
-  by (smt (verit) signed_0 signed_take_bit_int_less_self_iff sint_ge sint_word_ariths(4) word_sless_alt)
-
-lemma min_int:
-  fixes x :: "'a::len word"
-  assumes "x <s 0"
-  assumes "x \<noteq> (2^(LENGTH('a) - 1))"
-  shows "2^(LENGTH('a) - 1) <s x"
-  using assms sorry
-
-(*
-lemma min_int:
-  fixes x :: "'a::len word"
-  assumes "x <s 0 \<and> 0 <s x"
-  shows "x = 2^(LENGTH('a) - 1)"
-  using assms
-  using signed.less_asym by blast
-*)
-
-lemma negate_min_int:
-  fixes v :: "'a::len word"
-  assumes "v = (2^(LENGTH('a) - 1))"
-  shows "v = (-v)"
-  using assms
-  by (metis One_nat_def add.inverse_neutral double_eq_zero_iff mult_minus_right verit_minus_simplify(4))
-
-fun abs :: "'a::len word \<Rightarrow> 'a word" where
-  "abs x = (if x <s 0 then (-x) else x)"
-
-lemma
-  "abs(abs(x)) = abs(x)"
-  for x :: "'a::len word"
-proof (cases "0 \<le>s x")
-  case True
-  then show ?thesis
-    by force
-next
-  case neg: False
-  then show ?thesis
-  proof (cases "x = (2^LENGTH('a) - 1)")
-    case True
-    then show ?thesis
-      using negate_min_int
-      by (simp add: word_sless_alt)
-  next
-    case False
-    then show ?thesis using min_int negative_lower_bound
-      using negate_min_int by force
-  qed
-qed
-
-text \<open>We need to do the same proof at the value level.\<close>
-
-lemma invert_intval:
-  assumes "int_signed_value b v < 0"
-  assumes "b > 0 \<and> b \<le> 64"
-  assumes "take_bit b v = v"
-  assumes "v \<noteq> (2^(b - 1))"
-  shows "0 < int_signed_value b (-v)"
-  using assms apply simp sorry
-
-lemma negate_max_negative:
-  assumes "b > 0 \<and> b \<le> 64"
-  assumes "take_bit b v = v"
-  assumes "v = (2^(b - 1))"
-  shows "new_int b v = intval_negate (new_int b v)"
-  using assms apply simp using negate_min_int sorry
-
-lemma val_abs_always_pos:
-  assumes "b > 0 \<and> b \<le> 64"
-  assumes "take_bit b v = v"
-  assumes "v \<noteq> (2^(b - 1))"
-  assumes "intval_abs (new_int b v) = (new_int b v')"
-  shows "val_to_bool (val[(new_int b 0) < (new_int b v')]) \<or> val_to_bool (val[(new_int b 0) eq (new_int b v')])"
-proof (cases "v = 0")
-  case True
-  then have isZero: "intval_abs (new_int b 0) = new_int b 0"
-    by auto
-  then have "IntVal b 0 = new_int b v'"
-    using True assms by auto
-  then have "val_to_bool (val[(new_int b 0) eq (new_int b v')])"
-    by simp
-  then show ?thesis by simp
-next
-  case neq0: False
-  have zero: "int_signed_value b 0 = 0"
-    by simp
-  then show ?thesis
-  proof (cases "int_signed_value b v > 0")
-    case True
-    then have "val_to_bool(val[(new_int b 0) < (new_int b v)])"
-      using zero apply simp
-      by (metis One_nat_def ValueThms.signed_take_take_bit assms(1) val_bool_unwrap)
-    then have "val_to_bool (val[new_int b 0 < new_int b v'])"
-      by (metis assms(4) val_abs_pos)
-    then show ?thesis
-      by blast
-  next
-    case neg: False
-    then have "val_to_bool (val[new_int b 0 < new_int b v'])"
-    proof -
-      have "int_signed_value b v \<le> 0"
-        using assms neg neq0 by simp
-      then show ?thesis
-      proof (cases "int_signed_value b v = 0")
-        case True
-        then have "v = 0"
-          by (metis One_nat_def Suc_pred assms(1) assms(2) dual_order.refl int_signed_value.simps signed_eq_0_iff take_bit_of_0 take_bit_signed_take_bit)
-        then show ?thesis
-          using neq0 by simp
-      next
-        case False
-        then have "int_signed_value b v < 0"
-          using \<open>int_signed_value (b::nat) (v::64 word) \<sqsubseteq> (0::int)\<close> by linarith
-        then have "new_int b v' = new_int b (-v)"
-          using assms using intval_abs.elims
-          by simp
-        then have "0 < int_signed_value b (-v)"
-          using assms(3) invert_intval
-          using \<open>int_signed_value (b::nat) (v::64 word) < (0::int)\<close> assms(1) assms(2) by blast
-        then show ?thesis
-          using \<open>new_int (b::nat) (v'::64 word) = new_int b (- (v::64 word))\<close> assms(1) signed_eqiv zero by presburger
-      qed
-    qed
-    then show ?thesis
-      by simp
-  qed
-qed
-
-lemma intval_abs_elims:
-  assumes "intval_abs x \<noteq> UndefVal"
-  shows "\<exists>t v . x = IntVal t v \<and> 
-                    intval_abs x = new_int t (if int_signed_value t v < 0 then - v else v)"
-  by (meson intval_abs.elims assms)
-
-lemma wf_abs_new_int:
-  assumes "intval_abs (IntVal t v) \<noteq> UndefVal"
-  shows "intval_abs (IntVal t v) = new_int t v \<or> intval_abs (IntVal t v) = new_int t (-v)" 
-  by simp
-
-lemma mono_undef_abs:
-  assumes "intval_abs (intval_abs x) \<noteq> UndefVal"
-  shows "intval_abs x \<noteq> UndefVal"
-  using assms by force
-
-(* Value level proofs *)
-lemma val_abs_idem:
-  assumes "valid_value x (IntegerStamp b l h d u)"
-  assumes "val[abs(abs(x))] \<noteq> UndefVal"
-  shows "val[abs(abs(x))] = val[abs x]"
-proof -
-  obtain b v where in_def: "x = IntVal b v"
-    using assms intval_abs_elims mono_undef_abs by blast
-  then have bInRange: "b > 0 \<and> b \<le> 64"
-    using assms(1)
-    by (metis valid_stamp.simps(1) valid_value.simps(1))
-  then show ?thesis
-  proof (cases "int_signed_value b v < 0")
-    case neg: True
-    then show ?thesis
-    proof (cases "v = (2^(b - 1))")
-      case min: True
-      then show ?thesis
-        by (smt (z3) assms(1) bInRange in_def intval_abs.simps(1) intval_negate.simps(1) negate_max_negative new_int.simps valid_value.simps(1))
-    next
-      case notMin: False
-      then have nested: "(intval_abs x) = new_int b (-v)"
-        using neg val_abs_neg in_def by simp
-      also have "int_signed_value b (-v) > 0"
-        using neg notMin invert_intval bInRange
-        by (metis assms(1) in_def valid_value.simps(1))
-      then have "(intval_abs (new_int b (-v))) = new_int b (-v)"
-        by (smt (verit, best) ValueThms.signed_take_take_bit bInRange int_signed_value.simps intval_abs.simps(1) new_int.simps new_int_unused_bits_zero)
-      then show ?thesis
-        using nested by presburger
-    qed
-  next
-    case False
-    then show ?thesis
-      by (metis (mono_tags, lifting) assms(1) in_def intval_abs.simps(1) new_int.simps valid_value.simps(1))
-  qed
-qed
-
-(*
-lemma val_abs_negate:
-  assumes "intval_abs val[-x] \<noteq> UndefVal"
-  shows   "intval_abs val[-x] = intval_abs x"
-  using less_eq_def
-  by (metis (no_types, opaque_lifting) new_int.simps zero_neq_one take_bit_0 signed.less_linear 
-      signed.dual_order.strict_iff_not)
-*)
-
-paragraph \<open>Optimisations\<close>
-
-
-optimization AbsIdempotence:
-  when "wf_stamp x"
-  when "x..stamp() instanceof IntegerStamp"
-  "abs(abs(x)) \<longmapsto> abs(x)"
-  using val_abs_idem
-  using wf_stamp_def
-  by (smt (verit, best) EvalTreeE(4) is_IntegerStamp_def le_expr_def stamp_instanceof_IntegerStamp unary_eval.simps(1)) 
-
-value AbsIdempotence_code
-
-
-optimization AbsNegate: "(abs(-x)) \<longmapsto> abs(x)"
-  sorry
-  (*using val_abs_negate by auto*)
-
-value "(either (snd AbsIdempotence_code) (snd AbsNegate_code))"
-
+thm_oracles AbsNegation
 
 end (* End of AbsPhase *)
 
